NuLLReps.thy
@@ -261,8 +261,7 @@ lemma [\<nu>intro]: "\<nu>Zero (NuNatRound b) 0" unfolding \<nu>Zero_def by simp
     val num = Syntax.parse_term ctx num
     fun mk term = mk_nuTy (num, term) |> Syntax.check_term ctx |> Thm.cterm_of ctx
     val term = (
-        (dest_current_nu meta |> strip_binop_r \<^const_name>\<open>Separation\<close>
-            |> hd |> dest_RepSet |> #2 |> mk)
+        (dest_current_nu meta |> strip_separations |> hd |> dest_RepSet |> #2 |> mk)
       handle TERM _ => mk @{term \<open>\<nat>[32]\<close>}
         | ERROR _ => mk @{term \<open>\<nat>[32]\<close>}) |> @{print}
   in (NuSys.auto_construct ctx term meta, ctx)  end)
